use decide instead of bool_decide where possible

theories/heap_lang/lang.v
@@ -520,7 +520,7 @@ Definition bin_op_eval_bool (op : bin_op) (b1 b2 : bool) : option base_lit :=
 Definition bin_op_eval (op : bin_op) (v1 v2 : val) : option val :=
   if decide (op = EqOp) then
     (* Crucially, this compares the same way as [CmpXchg]! *)
-    if bool_decide (vals_compare_safe v1 v2) then
+    if decide (vals_compare_safe v1 v2) then
       Some $ LitV $ LitBool $ bool_decide (v1 = v2)
     else
       None
